Spec

specifications_formelles/tp4/tp4.v
@@ -2,14 +2,12 @@ Require Import FunInd.
 Require Import Omega.
 Open Scope list_scope.
 
-
-
 Inductive is_perm : (list nat) -> (list nat)  -> Prop :=
-  | is_perm_R : forall l1 : (list nat), is_perm l1 l1
+  | is_perm_R : forall l1 : (list nat),       is_perm l1 l1
   | is_perm_T : forall l1 l2 l3 : (list nat), is_perm l1 l2 -> is_perm l2 l3 -> is_perm l1 l3
-  | is_perm_S : forall l1 l2 : (list nat),  is_perm l1 l2 -> is_perm l2 l1
-  | is_perm_C : forall l1 l2 : (list nat),  forall a : nat, is_perm l1 l2 -> is_perm (a::l1) (a::l2)
-  | is_perm_A : forall l1 : (list nat),  forall a : nat, is_perm (a :: l1) (l1++ a::nil).
+  | is_perm_S : forall l1 l2 : (list nat),    is_perm l1 l2 -> is_perm l2 l1
+  | is_perm_C : forall l1 l2 : (list nat),    forall a : nat, is_perm l1 l2 -> is_perm (a::l1) (a::l2)
+  | is_perm_A : forall l1 : (list nat),       forall a : nat, is_perm (a :: l1) (l1++ a::nil).
 
 Definition l1  := 1::2::3::nil.
 Definition l2 := 3::2::1::nil.
@@ -46,20 +44,48 @@ omega.
 apply is_sort_1.
 Qed.
 
-Fixpoint insert (l : (list nat)) (n : nat) : (list nat):=
+Fixpoint insert (n : nat) (l : (list nat)) : (list nat):=
   match l with
     | nil => n::nil
     | h::tl => match le_dec n h with
       | left _ => n::h::tl
-      | right _ => h::(insert tl n)
+      | right _ => h::(insert n tl)
       end
     end.
 
 Fixpoint sort (l : (list nat)) : (list nat) :=
   match l with
     | nil => nil
-    | h::t => (insert (sort t) h)
+    | h::t => (insert  h (sort t))
     end.
+
+Theorem inter1:
+  forall (a1 : nat) (a2 : nat) (l : (list nat)), (is_perm (a1 :: a2 :: l) (a2 :: a1 :: l)).
+Proof.
+  intros.
+  apply (is_perm_T (a1::a2::l) (a2::l++a1::nil) (a2::a1::l)).
+  apply is_perm_A.
+  apply is_perm_C.
+  apply is_perm_S.
+  apply is_perm_A.
+Qed.
+
+Theorem perm_insert:
+  forall (a : nat) (l1 : (list nat)), (is_perm (a::l1) (insert a l1)).
+Proof.
+  induction l4.
+  simpl.
+  apply is_perm_A.
+  simpl.
+  elim (le_dec a0).
+  intros.
+  apply is_perm_R.
+  intros.
+  apply (is_perm_T (a0 :: a1 :: l4) (a1 :: a0 :: l4) (a1 :: insert a0 l4)).
+  apply inter1.
+  apply is_perm_C.
+  apply IHl4.
+
 
 Theorem yolo:
   forall (l1 l2 : (list nat)), (sort l1) = l2 -> (is_perm l1 l2) /\ is_sort(l2).
@@ -69,9 +95,9 @@ intros.
 split.
 simpl in H.
 rewrite <- H.
+(*
 apply is_perm_R.
 simpl in H.
 rewrite <- H.
 apply is_sort_O.
-
-
+*)
